src/program_proof/tulip/paxos/program/paxos_stepdown.v
@@ -55,7 +55,6 @@ Section stepdown.
     iDestruct (node_wal_fname_agree with "Hfnameme Hwalfname") as %->.
     iFrame "Hfile".
     iExists wal.
-    iSplit; first done.
     iIntros (bs') "[Hfile %Hbs']".
     iMod (paxos_inv_prepare (uint.nat term) with "Hwalfile Htermc Hterml Hlogn HinvO")
       as "(Hwalfile & Htermc & Hterml & Hlogn & HinvO & Hlsnp & #Hpromise)".
