src/program_proof/tulip/paxos/program/paxos_submit.v
@@ -89,7 +89,6 @@ Section submit.
     iDestruct (node_wal_fname_agree with "Hfnameme Hwalfname") as %->.
     iFrame "Hfile".
     iExists wal.
-    iSplit; first done.
     iIntros (bs') "[Hfile %Hbs']".
     iMod (paxos_inv_extend [c] with "[] Hps Hwalfile Htermc Hterml Hlogn HinvO")
       as "(Hps & Hwalfile & Htermc & Hterml & Hlogn & HinvO & #Hacpted')".
