src/program_proof/tulip/program/replica/replica_log.v
@@ -1,47 +1,198 @@
+From Perennial.program_proof Require Import marshal_stateless_proof.
 From Perennial.program_proof.tulip.program Require Import prelude.
+From Perennial.program_proof.tulip.program.util Require Import
+  encode_string encode_kvmap_from_slice.
 
 Section program.
   Context `{!heapGS Σ, !tulip_ghostG Σ}.
 
-  Theorem wp_Replica__logRead (rp : loc) (ts : u64) (key : string) :
-    {{{ True }}}
-      Replica__logRead #rp #ts #(LitString key)
-    {{{ RET #(); True }}}.
+  Theorem wp_logRead (fname : string) (ts : u64) (key : string) (bs : list u8) :
+    {{{ fname f↦ bs }}}
+      logRead #(LitString fname) #ts #(LitString key)
+    {{{ (bs' : list u8), RET #(); fname f↦ bs' }}}.
   Proof.
-    (*@ func (rp *Replica) logRead(ts uint64, key string) {                     @*)
-    (*@     // TODO: Create an inconsistent log entry for reading @key at @ts.  @*)
-    (*@ }                                                                       @*)
-  Admitted.
+    iIntros (Φ) "Hfile HΦ".
+    wp_rec.
 
-  Theorem wp_Replica__logValidate rp (ts : u64) (pwrsS : Slice.t) :
-    {{{ True }}}
-      Replica__logValidate #rp #ts (to_val pwrsS) slice.nil
-    {{{ RET #(); True }}}.
-  Proof.
-    (*@ func (rp *Replica) logValidate(ts uint64, pwrs []tulip.WriteEntry, ptgs []uint64) { @*)
-    (*@     // TODO: Create an inconsistent log entry for validating @ts with @pwrs and @ptgs. @*)
-    (*@ }                                                                       @*)
-  Admitted.
+    (*@ func logRead(fname string, ts uint64, key string) {                     @*)
+    (*@     // Create an inconsistent log entry for reading @key at @ts.        @*)
+    (*@     bs := make([]byte, 0, 32)                                           @*)
+    (*@                                                                         @*)
+    wp_apply wp_NewSliceWithCap; first word.
+    iIntros (p1) "Hbs".
+    rewrite uint_nat_W64_0 replicate_0.
 
-  Theorem wp_Replica__logFastPrepare (rp : loc) (ts : u64) (pwrs : Slice.t) :
-    {{{ True }}}
-      Replica__logFastPrepare #rp #ts (to_val pwrs) slice.nil
-    {{{ RET #(); True }}}.
-  Proof.
-    (*@ func (rp *Replica) logFastPrepare(ts uint64, pwrs []tulip.WriteEntry, ptgs []uint64) { @*)
-    (*@     // TODO: Create an inconsistent log entry for fast preparing @ts.   @*)
-    (*@ }                                                                       @*)
-  Admitted.
+    (*@     bs1 := marshal.WriteInt(bs, CMD_READ)                               @*)
+    (*@     bs2 := marshal.WriteInt(bs1, ts)                                    @*)
+    (*@     bs3 := util.EncodeString(bs2, key)                                  @*)
+    (*@                                                                         @*)
+    wp_apply (wp_WriteInt with "Hbs").
+    iIntros (p2) "Hbs".
+    wp_apply (wp_WriteInt with "Hbs").
+    iIntros (p3) "Hbs".
+    wp_apply (wp_EncodeString with "Hbs").
+    iIntros (p4) "Hbs".
+    wp_pures.
 
-  Theorem wp_Replica__logAccept (rp : loc) (ts : u64) (rank : u64) (dec : bool) :
-    {{{ True }}}
-      Replica__logAccept #rp #ts #rank #dec
-    {{{ RET #(); True }}}.
-  Proof.
-    (*@ func (rp *Replica) logAccept(ts uint64, rank uint64, dec bool) {        @*)
-    (*@     // TODO: Create an inconsistent log entry for accepting prepare decision @*)
-    (*@     // @dec for @ts in @rank.                                           @*)
+    (*@     grove_ffi.FileAppend(fname, bs3)                                    @*)
     (*@ }                                                                       @*)
-  Admitted.
+    wp_rec. wp_pures.
+    wp_rec. wp_pures.
+    wp_rec. wp_pures.
+    iDestruct (own_slice_to_small with "Hbs") as "Hbs".
+    iDestruct (own_slice_small_sz with "Hbs") as %Hszbs.
+    wp_apply (wp_FileAppendOp with "[$Hfile Hbs]").
+    { apply Hszbs. }
+    { iApply (own_slice_small_byte_pointsto_vals with "Hbs"). }
+    iIntros (err) "[Hfile Hbs]".
+    wp_pures.
+    destruct err; wp_pures.
+    { wp_apply wp_Exit. iIntros "[]". }
+    by iApply "HΦ".
+  Qed.
+
+  Theorem wp_logValidate
+    (fname : string) (ts : u64) (pwrsP : Slice.t) (pwrs : dbmap) (bs : list u8) :
+    {{{ fname f↦ bs ∗ own_dbmap_in_slice pwrsP pwrs }}}
+      logValidate #(LitString fname) #ts (to_val pwrsP) slice.nil
+    {{{ (bs' : list u8), RET #(); fname f↦ bs' ∗ own_dbmap_in_slice pwrsP pwrs }}}.
+  Proof.
+    iIntros (Φ) "[Hfile Hpwrs] HΦ".
+    wp_rec.
+
+    (*@ func logValidate(fname string, ts uint64, pwrs []tulip.WriteEntry, ptgs []uint64) { @*)
+    (*@     // Create an inconsistent log entry for validating @ts with @pwrs and @ptgs. @*)
+    (*@     bs := make([]byte, 0, 64)                                           @*)
+    (*@                                                                         @*)
+    wp_apply wp_NewSliceWithCap; first word.
+    iIntros (p1) "Hbs".
+    rewrite uint_nat_W64_0 replicate_0.
+
+    (*@     bs1 := marshal.WriteInt(bs, CMD_VALIDATE)                           @*)
+    (*@     bs2 := marshal.WriteInt(bs1, ts)                                    @*)
+    (*@     bs3 := util.EncodeKVMapFromSlice(bs2, pwrs)                         @*)
+    (*@                                                                         @*)
+    wp_apply (wp_WriteInt with "Hbs").
+    iIntros (p2) "Hbs".
+    wp_apply (wp_WriteInt with "Hbs").
+    iIntros (p3) "Hbs".
+    wp_apply (wp_EncodeKVMapFromSlice with "[$Hbs $Hpwrs]").
+    iIntros (p4 mdata) "[Hbs [Hpwrs %Hmdata]]".
+    wp_pures.
+
+    (*@     grove_ffi.FileAppend(fname, bs3)                                    @*)
+    (*@ }                                                                       @*)
+    wp_rec. wp_pures.
+    wp_rec. wp_pures.
+    wp_rec. wp_pures.
+    iDestruct (own_slice_to_small with "Hbs") as "Hbs".
+    iDestruct (own_slice_small_sz with "Hbs") as %Hszbs.
+    wp_apply (wp_FileAppendOp with "[$Hfile Hbs]").
+    { apply Hszbs. }
+    { iApply (own_slice_small_byte_pointsto_vals with "Hbs"). }
+    iIntros (err) "[Hfile Hbs]".
+    wp_pures.
+    destruct err; wp_pures.
+    { wp_apply wp_Exit. iIntros "[]". }
+    iApply "HΦ".
+    by iFrame.
+  Qed.
+
+  Theorem wp_logFastPrepare
+    (fname : string) (ts : u64) (pwrsP : Slice.t) (pwrs : dbmap) (bs : list u8) :
+    {{{ fname f↦ bs ∗ own_dbmap_in_slice pwrsP pwrs }}}
+      logFastPrepare #(LitString fname) #ts (to_val pwrsP) slice.nil
+    {{{ (bs' : list u8), RET #(); fname f↦ bs' ∗ own_dbmap_in_slice pwrsP pwrs }}}.
+  Proof.
+    iIntros (Φ) "[Hfile Hpwrs] HΦ".
+    wp_rec.
+
+    (*@ func logFastPrepare(fname string, ts uint64, pwrs []tulip.WriteEntry, ptgs []uint64) { @*)
+    (*@     // Create an inconsistent log entry for fast preparing @ts.         @*)
+    (*@     bs := make([]byte, 0, 64)                                           @*)
+    (*@                                                                         @*)
+    wp_apply wp_NewSliceWithCap; first word.
+    iIntros (p1) "Hbs".
+    rewrite uint_nat_W64_0 replicate_0.
+
+    (*@     bs1 := marshal.WriteInt(bs, CMD_FAST_PREPARE)                       @*)
+    (*@     bs2 := marshal.WriteInt(bs1, ts)                                    @*)
+    (*@     bs3 := util.EncodeKVMapFromSlice(bs2, pwrs)                         @*)
+    (*@                                                                         @*)
+    wp_apply (wp_WriteInt with "Hbs").
+    iIntros (p2) "Hbs".
+    wp_apply (wp_WriteInt with "Hbs").
+    iIntros (p3) "Hbs".
+    wp_apply (wp_EncodeKVMapFromSlice with "[$Hbs $Hpwrs]").
+    iIntros (p4 mdata) "[Hbs [Hpwrs %Hmdata]]".
+    wp_pures.
+
+    (*@     grove_ffi.FileAppend(fname, bs3)                                    @*)
+    (*@ }                                                                       @*)
+    wp_rec. wp_pures.
+    wp_rec. wp_pures.
+    wp_rec. wp_pures.
+    iDestruct (own_slice_to_small with "Hbs") as "Hbs".
+    iDestruct (own_slice_small_sz with "Hbs") as %Hszbs.
+    wp_apply (wp_FileAppendOp with "[$Hfile Hbs]").
+    { apply Hszbs. }
+    { iApply (own_slice_small_byte_pointsto_vals with "Hbs"). }
+    iIntros (err) "[Hfile Hbs]".
+    wp_pures.
+    destruct err; wp_pures.
+    { wp_apply wp_Exit. iIntros "[]". }
+    iApply "HΦ".
+    by iFrame.
+  Qed.
+
+  Theorem wp_logAccept (fname : string) (ts : u64) (rank : u64) (dec : bool) (bs : list u8) :
+    {{{ fname f↦ bs }}}
+      logAccept #(LitString fname) #ts #rank #dec
+    {{{ (bs' : list u8), RET #(); fname f↦ bs' }}}.
+  Proof.
+    iIntros (Φ) "Hfile HΦ".
+    wp_rec.
+
+    (*@ func logAccept(fname string, ts uint64, rank uint64, dec bool) {        @*)
+    (*@     // Create an inconsistent log entry for accepting prepare decision @dec for @*)
+    (*@     // @ts in @rank.                                                    @*)
+    (*@     bs := make([]byte, 0, 32)                                           @*)
+    (*@                                                                         @*)
+    wp_apply wp_NewSliceWithCap; first word.
+    iIntros (p1) "Hbs".
+    rewrite uint_nat_W64_0 replicate_0.
+
+    (*@     bs1 := marshal.WriteInt(bs, CMD_ACCEPT)                             @*)
+    (*@     bs2 := marshal.WriteInt(bs1, ts)                                    @*)
+    (*@     bs3 := marshal.WriteInt(bs2, rank)                                  @*)
+    (*@     bs4 := marshal.WriteBool(bs3, dec)                                  @*)
+    (*@                                                                         @*)
+    wp_apply (wp_WriteInt with "Hbs").
+    iIntros (p2) "Hbs".
+    wp_apply (wp_WriteInt with "Hbs").
+    iIntros (p3) "Hbs".
+    wp_apply (wp_WriteInt with "Hbs").
+    iIntros (p4) "Hbs".
+    wp_apply (wp_WriteBool with "Hbs").
+    iIntros (p5) "Hbs".
+    wp_pures.
+
+    (*@     grove_ffi.FileAppend(fname, bs4)                                    @*)
+    (*@ }                                                                       @*)
+    wp_rec. wp_pures.
+    wp_rec. wp_pures.
+    wp_rec. wp_pures.
+    iDestruct (own_slice_to_small with "Hbs") as "Hbs".
+    iDestruct (own_slice_small_sz with "Hbs") as %Hszbs.
+    wp_apply (wp_FileAppendOp with "[$Hfile Hbs]").
+    { apply Hszbs. }
+    { iApply (own_slice_small_byte_pointsto_vals with "Hbs"). }
+    iIntros (err) "[Hfile Hbs]".
+    wp_pures.
+    destruct err; wp_pures.
+    { wp_apply wp_Exit. iIntros "[]". }
+    iApply "HΦ".
+    by iFrame.
+  Qed.
 
 End program.
