src/program_proof/tulip/program/replica/replica_repr.v
@@ -126,9 +126,13 @@ Section repr.
       "%Hexec"      ∷ ⌜execute_cmds log = LocalState cm histm cpm ptgsm sptsm ptsm psm rkm⌝.
 
   Definition own_replica (rp : loc) (gid rid : u64) γ α : iProp Σ :=
-    ∃ (cloga : dblog) (lsna : u64),
+    ∃ (cloga : dblog) (lsna : u64) (fname : string) (bs : list u8),
       "Hrp"        ∷ own_replica_with_cloga_no_lsna rp cloga gid rid γ α ∗
       "Hlsna"      ∷ rp ↦[Replica :: "lsna"] #lsna ∗
+      "HfnameP"    ∷ rp ↦[Replica :: "fname"] #(LitString fname) ∗
+      (* TODO: The file pointsto really should be sealed in an atomic invariant,
+      but this won't be a problem until we start proving recovery. *)
+      "Hfile"      ∷ fname f↦ bs ∗
       "%Hlencloga" ∷ ⌜length cloga = uint.nat lsna⌝.
 
   Definition is_replica_idx (rp : loc) γ α : iProp Σ :=
